backend/ValueAnalysis.v
@@ -963,7 +963,7 @@ Proof.
   revert ARGS. generalize vargs.
   induction vargs0; simpl; intros; constructor.
   eapply vmatch_inj; eauto. auto.
-  intros (j' & vres' & m'' & EC' & IRES & IMEM & UNCH1 & UNCH2 & IINCR & ISEP).
+  intros (j' & vres' & m'' & EC' & IRES & IMEM & UNCH1 & UNCH2 & IINCR & ISEP & X).
   assert (JBELOW: forall b, sup_In b (Mem.support m) -> j' b = inj_of_bc bc b).
   {
     intros. destruct (inj_of_bc bc b) as [[b' delta] | ] eqn:EQ.
